proof/refine/StateRelationPre.thy
@@ -25,4 +25,17 @@ text \<open>
 type_synonym obj_relation_cut = "Structures_A.kernel_object \<Rightarrow> Structures_H.kernel_object \<Rightarrow> bool"
 type_synonym obj_relation_cuts = "(machine_word \<times> obj_relation_cut) set"
 
+text \<open>Arch object projection for predicates that depend on arch objects only.\<close>
+definition aobj_of':: "kernel_object \<Rightarrow> arch_kernel_object option" where
+  "aobj_of' ko \<equiv> case ko of KOArch ako \<Rightarrow> Some ako | _ \<Rightarrow> None"
+
+lemmas aobj_of'_simps[simp] = aobj_of'_def[split_simps kernel_object.split]
+
+lemma aobj_of'_Some[iff]:
+  "(aobj_of' a = Some ao) = (a = KOArch ao)"
+  by (simp add: aobj_of'_def split: kernel_object.splits)
+
+abbreviation aobjs_of' :: "kernel_state \<Rightarrow> obj_ref \<rightharpoonup> arch_kernel_object" where
+  "aobjs_of' \<equiv> \<lambda>s. ksPSpace s |> aobj_of'"
+
 end
