proof/refine/AARCH64/Untyped_R.thy
@@ -1393,6 +1393,7 @@ crunch set_cap, set_cdt
 crunch updateMDB, updateNewFreeIndex, setCTE
   for rdyq_projs[wp]:
     "\<lambda>s. P (ksReadyQueues s) (tcbSchedNexts_of s) (tcbSchedPrevs_of s) (\<lambda>d p. inQ d p |< tcbs_of' s)"
+  and aobjs_of'[wp]: "\<lambda>s. P (aobjs_of' s)"
 
 lemma insertNewCap_corres:
 notes if_cong[cong del] if_weak_cong[cong]
