proof/refine/ARM_HYP/ArchKHeap_R.thy
@@ -178,6 +178,11 @@ lemma obj_relation_cut_same_type:
 lemmas obj_at_simps = gen_obj_at_simps is_other_obj_relation_type_def
                       objBits_simps pageBits_def
 
+(* No aobjs dependency on this architecture *)
+lemma arch_state_relation_no_aobjs[elim!]:
+  "(s, s') \<in> arch_state_relation aobjs' \<Longrightarrow> (s, s') \<in> arch_state_relation aobjs"
+  by (simp add: arch_state_relation_def)
+
 lemma setObject_other_corres:
   fixes ob' :: "'a :: pspace_storable"
   assumes x: "updateObject ob' = updateObject_default ob'"
