proof/refine/RISCV64/ADT_H.thy
@@ -1456,7 +1456,7 @@ definition
 
 lemma absArchState_correct:
   "(s,s') \<in> state_relation \<Longrightarrow> absArchState (ksArchState s') = arch_state s"
-  apply (prop_tac "(arch_state s, ksArchState s') \<in> arch_state_relation")
+  apply (prop_tac "(arch_state s, ksArchState s') \<in> arch_state_relation (aobjs_of' s')")
    apply (simp add: state_relation_def)
   apply (clarsimp simp add: arch_state_relation_def)
   by (clarsimp simp add: absArchState_def
